\begin{frame}{Axioms}
\small \begin{align*}
(f^*g)^*(f^*z) &= f^*(g^*z)        && \mbox{$f \in inst(x),\ g \in inst(y),\ x < y$ and  $y < z$} \\
(f^*g)^*(f^*h) &= f^*(g^*h)        && \mbox{as above and $h \in inst(z)$ }\\
(x \cross y) \cross (x \cross z) &= x \cross (y \cross z)
                                   && \mbox{$x_c < y$, where $x_c \base x$, and $x_c < z$} \\
(x \cross y) \cross (x \cross g) &= x \cross (y \cross g)
                                   && \mbox{as above and $g \in inst(z)$}\\
f^*(x \cross y) &= y               && \mbox{ $f \in inst(x)$ and $x_c < y$, where $x_c \base x$}\\
f^*(x \cross g) &= g               && \mbox{as above and $g \in inst(y)$}\\
f^*y \cross f^*z &= f^*(y \cross z)  %problem here  
                    && \mbox{$f \in inst(x)$, $x < z$, $x < y$ and $y_c <z$ where $y_c \base y$}\\
f^*y \cross f^*g &= f^*(y \cross g)    && \mbox{as above  and $g \in inst(z)$}\\
(x \cross g)^*(x \cross z)&=x \cross(g^*z) && \mbox{$g \in inst(y)$ and $x_c < y$ and $y < z$, where $x_c \base x$}\\
(x \cross g)^*(x \cross h)&=x \cross(g^*h) && \mbox{as above and  $h \in inst(z)$}\\
\delta_x ^*(x \cross y)&=y                 && \mbox{$x < y$}\\
\delta_x ^*(x \cross g)&=g                 && \mbox{$x < y$ and $g\in inst(y)$}\\
f \sub \diag(x) &= f                       && \mbox{$f \in inst(x)$}\\
f \sub \diag(y) &= \diag(f \sub y)         && \mbox{$f \in inst(x)$ and  $x < y$.}
\end{align*}
\end{frame}