\begin{lemma}
\llabel{sofplemma}
If $1 \base y_1 ... \base b_m$ in \catc, for some $m \ge 1$ in a contextual category \catcw then \foreachj,
$s(p_{b_m,y_j}): b_m \morph \crossx{b_m}{y_j}{y_{j-1}}$ in \catcw.
\end{lemma}
\begin{proof}
Because $p_{b_m,y_j}: b_m \morph y_j$ in $\catcw$ and so be definition of operator $s$ it follows that $s(p_{b_m,y_j}): b_m  \morph (p_{b_m,y_j} \circ p_{y_j})^*y_j$
and we have 
\begin{align*}
(p_{b_m,y_j} \circ p_{y_j})^*y_j &= {p_{b_m,y_{j-1}}} ^*y_j  && \mbox{ because $p_{b_m,y_j} \circ p_{y_j}=p_{b_m,y_{j-1}}$,} \\
                                 &= \crossx{b_m}{y_j}{y_{j-1}} && \mbox{ by definition of $\crossx{}{}{w}$}.
\end{align*}
\end{proof}
\newpage
\begin{lemma}
\llabel{crosssectionlemma}
If 
\raisebox{-0.15cm}{
$
\begin{array}{ c c c}
\Rnode{y}{y} &              & \Rnode{Bp}{y'} \\[1cm]
             & \Rnode{x}{x} &     
\mbox{\nccdar{y}{x}
\ncsar{Bp}{x}
%\ncarr[-30]{x}{Bp}
\ncrightsimplesection{x}{Bp}
\blabel{g}}
\end{array}
$}
in a contextual category \catcw and if $g$ is a section of $y'$ (i.e. if $g \circ p_{y'}= id_x$) so that we have 
\begin{equation*}
\begin{array}{ c c c}
\Rnode{BBp}{\crossx{y}{y'}{x}} \\[1.3cm]
\Rnode{y}{y} &              & \Rnode{Bp}{y'} \\[1.1cm]
             & \Rnode{x}{x} &
\mbox{
\ncsar{BBp}{y}
\ncrightcrosssection{y}{BBp}
\blabel{\crossx{y}{g}{x}}
\nccdar{y}{x}
\blabel{p_{y,x}}
\ncsar{Bp}{x}
\ncrightsimplesection{x}{Bp}
\blabel{g}
\ncarr[30]{BBp}{Bp}
\alabel{q(p_{y,x},y')}
}                                                                                   
\end{array}
\end{equation*}
in \catcw,  then
\begin{equation}
\label{crosssectionlemmatarget}
\crossx{y}{g}{x} = s(p_{y,x} \circ g).
\end{equation} 
\end{lemma}
\begin{proof}
$\crossx{y}{g}{x}$ is defined to be the unique section of $\crossx{y}{y'}{x}$ such that $(\crossx{y}{g}{x}) \circ q( p_{y,x},y') = p_{y,x} \circ g$ and
so (\ref{crosssectionlemmatarget}) follows 
because $s(p_{y,x} \circ g)$ is a section of $\crossx{y}{y'}{x}$ (because by definition it is a section
of $(p_{y,x} \circ g \circ p_{y'}) ^*y'$ and this simplifies, because $g$ is a section, to  ${p_{y,x}} ^*y'$ i.e to $\crossx{y}{y'}{x}$ )
and because
$$s(p_{y,x} \circ g) \circ q( p_{y,x},y') = p_{y,x} \circ g$$
because
\begin{align*}
lhs &=  s(p_{y,x} \circ g) \circ q( p_{y,x} \circ g \circ p_{y'}, y') && \mbox{since $g$ is a section,} \\
    &=  p_{y,x} \circ g                                           && \mbox{by axiom (s2).} 
\end{align*}
\end{proof}
\newpage
\newcommand{\fsp}{f^*s(p_{y,x})}
\newcommand{\fyf}{\crossx{(f^*y)}{f}{x_p}}
\begin{lemma}
\llabel{missingsublemma3}
If $x_p$, $x$, $y_p$ and $y$ are objects of a contextual category \catcw such that
$x_P \base x \leq y_p \base y$ and if $f \in Sect(x)$ then
$$\fsp = \fyf$$
as shown here:
\begin{displaymath}
\newcommand{\yx}{\crossx{y}{x}{x_p}}
\newcommand{\fyx}{\crossx{(f^*y)}{x}{x_p}}
\newcommand{\spyx}{s(p_{y,x})}
\begin{array}{c p{0.5cm} c p{0.5cm} c} 
                    &&                 && \Rnode{yx}{\yx}            \\[1.4cm]
\Rnode{fyx}{\fyx}   &&                 && \Rnode{y}{y}               \\[1.4cm]
\Rnode{fy}{f^*y}    &&                 && \Rnode{yp}{y_p}            \\[1.2cm]
\Rnode{fyp}{f^*y_p} &&                 &&                            \\[1.8cm]
                    && \Rnode{x}{x}    &&                            \\[1.2cm]
                    && \Rnode{xp}{x_p} &&   
\makebox[0cm]{
\ncsar{yx}{y}
\ncarc[arcangle=15,nodesepA=5pt,offsetA=4pt,nodesepB=3pt,offsetB=2pt]{->}{y}{yx}
\alabel{\spyx} [0.4]
\ncsar{y}{yp}
\nccdar{yp}{x}
\ncsar{x}{xp}
\ncarc[arcangle=-15,nodesepA=5pt,offsetA=-2pt,nodesepB=3pt,offsetB=-2pt]{->}{xp}{x}
\blabel{f} [0.5]
\ncsar{fyx}{fy}
\ncarc[arcangle=15,nodesepA=5pt,offsetA=4pt,nodesepB=3pt,offsetB=2pt]{->}{fy}{fyx}
\alabel{f^*(\spyx)=\fyf} [0.4]
\ncsar{fy}{fyp}
\nccdar{fyp}{xp}
\ncarr{fyx}{yx}
\alabel{q(f,\yx)}[0.5][-4]
\ncarr{fy}{y}
\alabel{q(f,y)}[0.45][-1]
\ncarr{fyp}{yp}
\alabel{q(f,y_p)}[0.5][-1]
}
\end{array}
\end{displaymath}
\end{lemma}
\begin{proof}
\begin{align*}
\fsp &= q(f,y)^*s(p_{y,x})           && \mbox{ by definition of extended $^*$,} \\
     &= s(q(f,y)\circ s(p_{y,x}))    && \mbox{by lemma \lref{regardingfstarsection},}  \\
     &= s(q(f,y)\circ p_{y,x})       && \mbox{ by lemma \lref{sfglemma},}  \\
     &= s(p_{f^*y,x_p} \circ f)      && \mbox{ because pullback diagram commutes,}  \\
     &= \fyf                         && \mbox{ by lemma  \lref{crosssectionlemma}.}
\end{align*}
\end{proof}
\newpage

\begin{lemma}
\llabel{sofpsubstitutionlemma}
If $1 \base x_1 ... \base x_n \base x_{n+1}$, for some $n \ge 1$ in a contextual category \catc, then 
for each $i$ and $j$, $1 \leq i < j \leq n+1$
\begin{equation*}
s(p_{x_{n},x_{i}})^*...s(p_{x_{n},x_1})^*(\crossx{x_{n}}{x_j}{1}) 
= \crossx{x_{n}}{x_j}{x_{i}}.
\end{equation*} 
\end{lemma}
\begin{proof}
By induction on $i$. 
In the case of $i=1$ we have 
\begin{align*}
s(p_{x_n,x_1})^*(\crossx{x_{n}}{x_j}{1})
& = s(p_{x_n,x_1}) ^* {p_{x_n,1}} ^* x_j
&&\mbox{ by definition of $\crossx{}{}{}$}\\
&= s(p_{x_{n},x_{i}})^*  q(p_{x_n,1},x_1) ^* x_j
&&\mbox{ by definition of extended $^*$,}\\
&= (s(p_{x_{n},x_1}) \circ q(p_{x_n,1},x_1)) ^* x_j
&&\mbox{ by (q5),}\\
&= {p_{x_{n},x_1}}^*x_j
&&\mbox{ by (s2),} \\
&= \crossx{x_{n}}{x_j}{x_1}
&&\mbox{by definition of $\crossx{}{}{}$, as required.}
\end{align*}
If $i >1$ then we have the following diagram in \catc 
$$
\begin{array}{cp{0.5cm}cc}
\Rnode{L0}{{p_{x_n,x_{i-1}}}^*x_j} &&                 &                \\[1.0cm]
\Rnode{L1}{{p_{x_n,x_{i-1}}}^*x_i} &&                 &                \\[1.0cm]
\Rnode{L2}{x_n}                    &&                 &                \\[0.25cm]
                                   && \Rnode{L3}{x_j} &                \\[1.0cm]
                                   && \Rnode{L4}{x_i} &                \\[0.5cm]
\Rnode{L5}{x_{i-1}}                &&                 &           
\end{array}
\mbox{
\nccdar{L0}{L1} 
\ncsar{L1}{L2}  
\nccdar{L2}{L5}   
\nccdar{L3}{L4}   
\ncsar{L4}{L5}
\ncarr[-10]{L1}{L4}
\alabel{q(p_{x_n,x_{i-1}},x_i)}[0.35]
\ncleftsimplesection{L2}{L1}
\alabel{s(p_{x_n,x_i})}
}
$$
and we can show
\begin{align*}
s(p_{x_{n},x_{i}})^*...s(p_{x_{n},x_1})^*(\crossx{x_{n}}{x_j}{1})
& = s(p_{x_{n},x_{i}})^* (\crossx{x_{n}}{x_j}{x_{i-1}})
&&\mbox{ by the inductive hypthesis,} \\
&= s(p_{x_{n},x_{i}})^* {p_{x_n,x_{i-1}}} ^* x_j
&&\mbox{ by definition of $\crossx{}{}{}$,}\\
&= s(p_{x_{n},x_{i}})^*  q(p_{x_n,x_{i-1}},x_i) ^* x_j
&&\mbox{ by definition of extended $^*$,}\\
&= (s(p_{x_{n},x_{i}}) \circ q(p_{x_n,x_{i-1}},x_i)) ^* x_j
&&\mbox{ by (q5),}\\
&= {p_{x_{n},x_{i}}}^*x_j
&&\mbox{ by (s2),} \\
&= \crossx{x_{n}}{x_j}{x_{i}}
&&\mbox{by definition of $\crossx{}{}{}$, as required.}
\end{align*}
\end{proof}
\begin{aside}
This above proof could be made more concise by extending the $^*$ operation to be such that if $f: x \morph y$ in \catcw then $f^*y$ is defined to by $y$. 
\end{aside}